fixed and added new invariants

src/dvspec/dafny/att_spec_proofs/inv.dfy
@@ -13,9 +13,9 @@ module AttInvariants
     import opened DVCNode_Spec
     import opened DV
 
-    predicate no_conflict_decisions_in_sec_3_1<D(!new, 0)>()
+    predicate no_conflict_decisions_pred1_in_sec_3_1<D(!new, 0)>(s: ConsensusInstance<D>)
     {
-        forall s: ConsensusInstance<D>, i1: BLSPubkey, i2: BLSPubkey | 
+        forall i1: BLSPubkey, i2: BLSPubkey | 
             && ConsensusSpec.isConditionForSafetyTrue(s)
             && i1 in s.honest_nodes_status.Keys
             && i2 in s.honest_nodes_status.Keys ::                         
@@ -24,10 +24,9 @@ module AttInvariants
                     || s.honest_nodes_status[i1] == s.honest_nodes_status[i2]
     }
 
-    predicate no_decisions_pred_in_sec_3_1<D(!new, 0)>()
+    predicate no_decisions_pred2_in_sec_3_1<D(!new, 0)>(s: ConsensusInstance<D>)
     {
-        forall s: ConsensusInstance<D> ::
-            ConsensusSpec.isConditionForSafetyTrue(s)
+        ConsensusSpec.isConditionForSafetyTrue(s)
                 ==> ( !s.decided_value.isPresent()
                         <==> ( forall i: BLSPubkey | i in s.honest_nodes_status.Keys ::
                                     s.honest_nodes_status[i] == NOT_DECIDED
@@ -42,9 +41,9 @@ module AttInvariants
         && n in s.honest_nodes_states.Keys
     }
 
-    predicate consistant_att_slashing_databases_between_honest_nodes_in_sec_3_2<D(!new, 0)>()
+    predicate consistant_att_slashing_databases_between_honest_nodes_pred3_in_sec_3_2<D(!new, 0)>(s: DVState)
     {
-        forall s: DVState, n1: BLSPubkey, n2: BLSPubkey |
+        forall n1: BLSPubkey, n2: BLSPubkey |
             && is_honest_node(s, n1)
             && is_honest_node(s, n2) 
                 :: || s.honest_nodes_states[n1].attestation_slashing_db <= s.honest_nodes_states[n2].attestation_slashing_db
@@ -52,154 +51,119 @@ module AttInvariants
                    
     }
 
-    predicate consistant_attestations_in_one_slashing_db_in_sec_3_2<D(!new, 0)>()
+    predicate consistant_attestations_in_one_slashing_db_pred4_in_sec_3_2<D(!new, 0)>(dvn: DVState)
     {
-        forall s: DVState,
-               pubkey: BLSPubkey, 
-               nState: DVCNodeState,
-               att: SlashingDBAttestation, 
-               att_data: AttestationData, 
-               att_duty: AttestationDuty |
-            && is_honest_node(s, pubkey)
-            && nState == s.honest_nodes_states[pubkey]
-            && att in nState.attestation_slashing_db
-            && att_duty in nState.all_rcvd_duties
-            && att.signing_root == Some(hash_tree_root(att_data))
-            && att_data.slot == att_duty.slot ::
-                    consensus_is_valid_attestation_data(nState.attestation_slashing_db, att_data, att_duty)         
+        forall pubkey: BLSPubkey | is_honest_node(dvn, pubkey) ::
+            && var nState := dvn.honest_nodes_states[pubkey];
+            && var db := nState.attestation_slashing_db;
+            && forall att: SlashingDBAttestation | att in db ::
+                    exists att_data: AttestationData, 
+                           att_duty: AttestationDuty ::
+                                && att_duty in nState.all_rcvd_duties
+                                && att.signing_root == Some(hash_tree_root(att_data))            
+                                && att_data.slot == att_duty.slot 
+                                && consensus_is_valid_attestation_data(db, att_data, att_duty)         
     }
 
-    predicate curr_att_duty_is_last_served_duty_in_sec_3_3<D(!new, 0)>()        
+    predicate curr_att_duty_is_last_served_duty_pred5_in_sec_3_3<D(!new, 0)>(dvn: DVState)        
     {
-        forall dvn: DVState,
-               pubkey: BLSPubkey,
-               s: DVCNodeState | 
-                    && is_honest_node(dvn, pubkey)
-                    && s == dvn.honest_nodes_states[pubkey] :: 
-                            s.current_attestation_duty.isPresent()
-                                ==> ( && s.latest_attestation_duty.isPresent()
-                                      && s.current_attestation_duty.safe_get() == s.latest_attestation_duty.safe_get()
-                                    )
+        forall pubkey: BLSPubkey | is_honest_node(dvn, pubkey) ::
+            && var s := dvn.honest_nodes_states[pubkey];
+            && s.current_attestation_duty.isPresent()
+                    ==> ( && s.latest_attestation_duty.isPresent()
+                          && s.current_attestation_duty.safe_get() == s.latest_attestation_duty.safe_get()
+                        )
     }
 
-    predicate exisiting_consensus_instance_for_curr_att_duty_in_sec_3_3<D(!new, 0)>()        
+    predicate exisiting_consensus_instance_for_curr_att_duty_pred6_in_sec_3_3<D(!new, 0)>(dvn: DVState)        
     {
-        forall dvn: DVState,
-               pubkey: BLSPubkey,
-               s: DVCNodeState | 
-                    && is_honest_node(dvn, pubkey)
-                    && s == dvn.honest_nodes_states[pubkey] ::
-                        s.current_attestation_duty.isPresent()
-                                ==> ( s.current_attestation_duty.safe_get().slot 
-                                        in s.attestation_consensus_engine_state.attestation_consensus_active_instances.Keys )
+        forall pubkey: BLSPubkey | is_honest_node(dvn, pubkey) ::
+            && var s := dvn.honest_nodes_states[pubkey];
+            && s.current_attestation_duty.isPresent()
+                    ==> s.current_attestation_duty.safe_get().slot 
+                            in s.attestation_consensus_engine_state.attestation_consensus_active_instances.Keys 
     }
 
-    predicate active_consensus_instances_imples_existence_of_curr_att_duty_in_sec_3_3<D(!new, 0)>()        
+    predicate active_consensus_instances_imples_existence_of_curr_att_duty_pred7_in_sec_3_3<D(!new, 0)>(dvn: DVState)        
     {
-        forall dvn: DVState,
-               pubkey: BLSPubkey,
-               s: DVCNodeState | 
-                    && is_honest_node(dvn, pubkey)
-                    && s == dvn.honest_nodes_states[pubkey] ::
-                        s.attestation_consensus_engine_state.attestation_consensus_active_instances.Keys != {}
-                            ==> ( && s.current_attestation_duty.isPresent()
-                                  && s.current_attestation_duty.safe_get().slot 
-                                        in s.attestation_consensus_engine_state.attestation_consensus_active_instances.Keys 
-                    )
+        forall pubkey: BLSPubkey | is_honest_node(dvn, pubkey) ::
+            && var s := dvn.honest_nodes_states[pubkey];
+            && s.attestation_consensus_engine_state.attestation_consensus_active_instances.Keys != {}
+                    ==> ( && s.current_attestation_duty.isPresent()
+                          && s.current_attestation_duty.safe_get().slot 
+                                in s.attestation_consensus_engine_state.attestation_consensus_active_instances.Keys 
+                        )
     }
     
-    predicate queued_duties_later_than_curr_att_duty_in_sec_3_3<D(!new, 0)>()        
+    predicate queued_duties_later_than_curr_att_duty_pred8_in_sec_3_3<D(!new, 0)>(dvn: DVState)        
     {
-        forall dvn: DVState,
-               pubkey: BLSPubkey,
-               s: DVCNodeState | 
-                    && is_honest_node(dvn, pubkey)
-                    && s == dvn.honest_nodes_states[pubkey] ::
-                        s.current_attestation_duty.isPresent()
-                            ==> forall queued_duty: AttestationDuty |
-                                    queued_duty in s.attestation_duties_queue :: 
-                                        s.current_attestation_duty.safe_get().slot < queued_duty.slot
+        forall pubkey: BLSPubkey | is_honest_node(dvn, pubkey) ::
+            && var s := dvn.honest_nodes_states[pubkey];
+            && s.current_attestation_duty.isPresent()
+                    ==> forall queued_duty: AttestationDuty | queued_duty in s.attestation_duties_queue :: 
+                            s.current_attestation_duty.safe_get().slot < queued_duty.slot
     }
 
-    predicate submitted_att_by_curr_att_duty_in_sec_3_3<D(!new, 0)>()        
+    predicate submitted_att_by_curr_att_duty_pred9_in_sec_3_3<D(!new, 0)>(dvn: DVState)        
     {
-        forall dvn: DVState,
-               pubkey: BLSPubkey,
-               s: DVCNodeState | 
-                    && is_honest_node(dvn, pubkey)
-                    && s == dvn.honest_nodes_states[pubkey] ::
-                        s.current_attestation_duty.isPresent()
-                            ==> (forall i: nat | 0 <= i && i < |s.bn.attestations_submitted| ::
-                                    s.bn.attestations_submitted[i].data.slot <= s.current_attestation_duty.safe_get().slot)            
+        forall pubkey: BLSPubkey | is_honest_node(dvn, pubkey) ::
+            && var s := dvn.honest_nodes_states[pubkey];
+            && s.current_attestation_duty.isPresent()
+                    ==> forall i: nat | 0 <= i && i < |s.bn.attestations_submitted| ::
+                            s.bn.attestations_submitted[i].data.slot <= s.current_attestation_duty.safe_get().slot
     }
 
-    predicate none_latest_att_duty_implies_empty_att_duty_queue_in_sec_3_4<D(!new, 0)>()        
+    predicate none_latest_att_duty_implies_empty_att_duty_queue_pred10_in_sec_3_4<D(!new, 0)>(dvn: DVState)        
     {
-        forall dvn: DVState,
-               pubkey: BLSPubkey,
-               s: DVCNodeState | 
-                    && is_honest_node(dvn, pubkey)
-                    && s == dvn.honest_nodes_states[pubkey] ::
-                        !s.latest_attestation_duty.isPresent()
-                            ==> |s.attestation_duties_queue| == 0
+        forall pubkey: BLSPubkey | is_honest_node(dvn, pubkey) ::
+            && var s := dvn.honest_nodes_states[pubkey];
+            && !s.latest_attestation_duty.isPresent()
+                    ==> |s.attestation_duties_queue| == 0
     }
 
-    predicate queued_duties_later_than_latest_att_duty_in_sec_3_4<D(!new, 0)>()        
+    predicate queued_duties_later_than_latest_att_duty_pred11_in_sec_3_4<D(!new, 0)>(dvn: DVState)        
     {
-        forall dvn: DVState,
-               pubkey: BLSPubkey,
-               s: DVCNodeState | 
-                    && is_honest_node(dvn, pubkey)
-                    && s == dvn.honest_nodes_states[pubkey] ::
-                        s.latest_attestation_duty.isPresent()
-                            ==> forall queued_duty: AttestationDuty |
-                                    queued_duty in s.attestation_duties_queue :: 
-                                        s.latest_attestation_duty.safe_get().slot < queued_duty.slot
+        forall pubkey: BLSPubkey | is_honest_node(dvn, pubkey) ::
+            && var s := dvn.honest_nodes_states[pubkey];
+            && s.latest_attestation_duty.isPresent()
+                    ==> forall queued_duty: AttestationDuty | queued_duty in s.attestation_duties_queue :: 
+                            s.latest_attestation_duty.safe_get().slot < queued_duty.slot
     }
 
-    predicate submitted_att_by_latest_att_duty_in_sec_3_4<D(!new, 0)>()        
+    predicate submitted_att_by_latest_att_duty_pred12_in_sec_3_4<D(!new, 0)>(dvn: DVState)        
     {
-        forall dvn: DVState,
-               pubkey: BLSPubkey,
-               s: DVCNodeState | 
-                    && is_honest_node(dvn, pubkey)
-                    && s == dvn.honest_nodes_states[pubkey] ::
-                        s.latest_attestation_duty.isPresent()
-                            ==> (forall i: nat | 0 <= i && i < |s.bn.attestations_submitted| ::
-                                    s.bn.attestations_submitted[i].data.slot <= s.latest_attestation_duty.safe_get().slot)            
+        forall pubkey: BLSPubkey | is_honest_node(dvn, pubkey) ::
+            && var s := dvn.honest_nodes_states[pubkey];
+            && s.latest_attestation_duty.isPresent()
+                    ==> forall i: nat | 0 <= i && i < |s.bn.attestations_submitted| ::
+                            s.bn.attestations_submitted[i].data.slot <= s.latest_attestation_duty.safe_get().slot
     }
 
-    predicate active_consensus_instances_for_slots_until_latest_att_duty_in_sec_3_4<D(!new, 0)>()        
+    predicate active_consensus_instances_for_slots_until_latest_att_duty_pred13_in_sec_3_4<D(!new, 0)>(dvn: DVState)        
     {
-        forall dvn: DVState,
-               pubkey: BLSPubkey,
-               s: DVCNodeState | 
-                    && is_honest_node(dvn, pubkey)
-                    && s == dvn.honest_nodes_states[pubkey] ::
-                        s.latest_attestation_duty.isPresent()
-                            ==> ( forall i: Slot | i in s.attestation_consensus_engine_state.attestation_consensus_active_instances.Keys ::
-                                        i <= s.latest_attestation_duty.safe_get().slot )
+        forall pubkey: BLSPubkey | is_honest_node(dvn, pubkey) ::
+            && var s := dvn.honest_nodes_states[pubkey];
+            && s.latest_attestation_duty.isPresent()
+                    ==> forall i: Slot | i in s.attestation_consensus_engine_state.attestation_consensus_active_instances.Keys ::
+                            i <= s.latest_attestation_duty.safe_get().slot
     }
 
-    predicate no_active_consensus_instances_for_queued_att_duties_in_sec_3_5<D(!new, 0)>()        
+    predicate no_active_consensus_instances_for_queued_att_duties_pred14_in_sec_3_5<D(!new, 0)>(dvn: DVState)        
     {
-        forall dvn: DVState,
-               pubkey: BLSPubkey,
-               s: DVCNodeState,
-               i: Slot, 
-               j: nat | 
-                    && is_honest_node(dvn, pubkey)
-                    && s == dvn.honest_nodes_states[pubkey] 
+        forall pubkey: BLSPubkey | is_honest_node(dvn, pubkey) ::
+            && var s := dvn.honest_nodes_states[pubkey];
+            && forall i: Slot, j: nat | 
                     && i in s.attestation_consensus_engine_state.attestation_consensus_active_instances.Keys 
                     && 0 <= j
                     && j < |s.attestation_duties_queue| ::
-                        i <= s.attestation_duties_queue[j].slot
+                        i < s.attestation_duties_queue[j].slot
     }
 
-    predicate at_most_one_active_consensus_instances_has_not_decided_in_sec_3_5<D(!new, 0)>()        
+    /*
+    // Seems wrong
+    predicate at_most_one_active_consensus_instances_has_not_decided_pred15_in_sec_3_5<D(!new, 0)>(dvn: DVState)        
     {
-        forall dvn: DVState,
-               pubkey: BLSPubkey,
+        forall pubkey: BLSPubkey,
                s: DVCNodeState,
                i: Slot, 
                j: Slot   | 
@@ -210,49 +174,72 @@ module AttInvariants
                     && j < |s.attestation_duties_queue| ::
                         i <= s.attestation_duties_queue[j].slot
     }
+    */
 
-    predicate att_from_imported_block_is_decided_value_in_sec_3_6<D(!new, 0)>()        
+    predicate att_from_imported_block_is_decided_value_pred16_in_sec_3_6<D(!new, 0)>(dvn: DVState)        
     {
-        forall dvn: DVState,
-               pubkey: BLSPubkey,
-               s: DVCNodeState,
-               i: nat,
-               slot: Slot  | 
-                    && is_honest_node(dvn, pubkey)
-                    && s == dvn.honest_nodes_states[pubkey] 
-                    && i in s.attestation_consensus_engine_state.attestation_consensus_active_instances.Keys 
+        forall pubkey: BLSPubkey | is_honest_node(dvn, pubkey) ::
+            && var s := dvn.honest_nodes_states[pubkey];
+            && forall i: nat |                     
+                    // && i in s.attestation_consensus_engine_state.attestation_consensus_active_instances.Keys 
                     && 0 <= i
-                    && i < |s.bn.attestations_submitted|
-                    && slot == s.bn.attestations_submitted[i].data.slot ::
+                    && i < |s.bn.attestations_submitted| ::
+                        && var slot := s.bn.attestations_submitted[i].data.slot;
                         && dvn.consensus_on_attestation_data[slot].decided_value.isPresent()
                         && s.bn.attestations_submitted[i].data == dvn.consensus_on_attestation_data[slot].decided_value.safe_get()
     }
 
-    predicate AttConsensusDecided_is_decided_value_in_sec_3_7<D(!new, 0)>()        
+    predicate old_duty_has_submitted_att_data_pred17_in_sec_3_6<D(!new, 0)>(dvn: DVState)        
     {
-        forall dvn: DVState,
-               pubkey: BLSPubkey,
-               s: DVCNodeState,
-               s': DVCNodeState,               
-               slot: Slot,
-               att_data: AttestationData  | 
-                    && is_honest_node(dvn, pubkey)
-                    && s == dvn.honest_nodes_states[pubkey] 
-                    && f_att_consensus_decided.requires(s, slot, att_data)
-                    && s' == f_att_consensus_decided(s, slot, att_data).state ::
+        forall pubkey: BLSPubkey | is_honest_node(dvn, pubkey) ::
+            && var s := dvn.honest_nodes_states[pubkey];            
+            && s.latest_attestation_duty.isPresent()
+            && forall duty: AttestationDuty |
+                    && duty in s.all_rcvd_duties      
+                    && duty.slot < s.latest_attestation_duty.safe_get().slot ::
+                            exists j: nat ::
+                                && 0 <= j
+                                && j < |s.bn.attestations_submitted| 
+                                && duty.slot == s.bn.attestations_submitted[j].data.slot
+    }
+
+    predicate AttConsensusDecided_is_decided_value_pred18_in_sec_3_7<D(!new, 0)>(dvn: DVState)        
+    {
+        forall pubkey: BLSPubkey | is_honest_node(dvn, pubkey) ::
+            && var s := dvn.honest_nodes_states[pubkey];
+            && forall slot: Slot, att_data: AttestationData | 
+                    f_att_consensus_decided.requires(s, slot, att_data) ::
+                        // && var s' := f_att_consensus_decided(s, slot, att_data).state;
+                        && slot in dvn.consensus_on_attestation_data.Keys
                         && dvn.consensus_on_attestation_data[slot].decided_value.isPresent()
                         && dvn.consensus_on_attestation_data[slot].decided_value.safe_get() == att_data                        
     }
 
-    predicate strictly_monotonic_att_duties_queue_in_sec_3_7<D(!new, 0)>()        
+    predicate local_active_consensus_instance_not_later_than_latest_duty_pred19a_in_sec_3_7<D(!new, 0)>(dvn: DVState)        
     {
-        forall dvn: DVState,
-               pubkey: BLSPubkey,
-               s: DVCNodeState,               
-               i1: nat,
-               i2: nat | 
-                    && is_honest_node(dvn, pubkey)
-                    && s == dvn.honest_nodes_states[pubkey] 
+        forall pubkey: BLSPubkey | is_honest_node(dvn, pubkey) ::
+            && var s := dvn.honest_nodes_states[pubkey];
+            && s.latest_attestation_duty.isPresent()
+                ==> forall slot: Slot | slot in s.attestation_consensus_engine_state.attestation_consensus_active_instances.Keys ::    
+                        slot <= s.latest_attestation_duty.safe_get().slot
+    }
+
+    predicate no_latest_duty_is_older_than_distributed_undecided_consensus_instance_pred19b_in_sec_3_7<D(!new, 0)>(dvn: DVState)        
+    {        
+        forall slot: Slot | slot in dvn.consensus_on_attestation_data.Keys ::
+            !dvn.consensus_on_attestation_data[slot].decided_value.isPresent()
+                ==> ( forall pubkey: BLSPubkey | is_honest_node(dvn, pubkey) ::
+                        && var s := dvn.honest_nodes_states[pubkey];
+                        && s.latest_attestation_duty.isPresent()
+                            ==> s.latest_attestation_duty.safe_get().slot <= slot
+                    )
+    }
+
+    predicate strictly_monotonic_att_duties_queue_pred20_in_sec_3_7<D(!new, 0)>(dvn: DVState)        
+    {
+        forall pubkey: BLSPubkey | is_honest_node(dvn, pubkey) ::
+            && var s := dvn.honest_nodes_states[pubkey];
+            && forall i1: nat, i2: nat | 
                     && 0 <= i1
                     && i1 < |s.attestation_duties_queue|
                     && 0 <= i2
@@ -283,82 +270,74 @@ module AttInvariants
                     && fork_version == bn_get_fork_version(att_data.slot)                                                                                
     }
 
-    predicate constructable_set_of_att_shares_has_at_least_one_share_from_honest_node_in_sec_3_7<D(!new, 0)>()        
+    predicate constructable_set_of_att_shares_has_at_least_one_share_from_honest_node_pred21_in_sec_3_7<D(!new, 0)>(dvn: DVState)        
     {
-        forall dvn: DVState,
-               pubkey: BLSPubkey,
-               s: DVCNodeState,               
-               slot: Slot,
-               att_data: AttestationData,
-               att_shares: set<AttestationShare>,
-               aggregation_bits: seq<bool> | 
-                    && is_honest_node(dvn, pubkey)
-                    && s == dvn.honest_nodes_states[pubkey]
-                    && slot in s.rcvd_attestation_shares.Keys
-                    && (att_data, aggregation_bits) in s.rcvd_attestation_shares[slot].Keys
-                    && att_data.slot == slot
-                    && att_shares == s.rcvd_attestation_shares[slot][(att_data, aggregation_bits)]
-                    && s.construct_signed_attestation_signature(att_shares).isPresent()
-                    && ( forall share: AttestationShare | share in att_shares :: share.data == att_data ) ::
-                            exists pubkey1: BLSPubkey,
-                            s1: DVCNodeState ::
-                                    && is_honest_node(dvn, pubkey1)
-                                    && s1 == dvn.honest_nodes_states[pubkey1]
-                                    && existing_share_from_node(att_shares, att_data, s1, slot)                                   
+        forall pubkey: BLSPubkey | is_honest_node(dvn, pubkey) ::
+            && var s := dvn.honest_nodes_states[pubkey];
+            && forall slot: Slot,
+                      att_data: AttestationData,
+                      att_shares: set<AttestationShare>,
+                      aggregation_bits: seq<bool> | 
+                            && slot in s.rcvd_attestation_shares.Keys
+                            && (att_data, aggregation_bits) in s.rcvd_attestation_shares[slot].Keys
+                            && att_data.slot == slot
+                            && att_shares == s.rcvd_attestation_shares[slot][(att_data, aggregation_bits)] ::
+                                    s.construct_signed_attestation_signature(att_shares).isPresent()
+                                        ==>  exists share: AttestationShare,
+                                                    pubkey1: BLSPubkey :: 
+                                                        && share in att_shares 
+                                                        && share.data == att_data                                                     
+                                                        && is_honest_node(dvn, pubkey1)
+                                                        && var s1 := dvn.honest_nodes_states[pubkey1];
+                                                        && existing_share_from_node(att_shares, att_data, s1, slot)                                      
     }
 
-    predicate no_missing_att_in_db_cond1_in_sec_3_7<D(!new, 0)>()        
+    predicate no_missing_att_in_db_pred21_in_sec_3_7<D(!new, 0)>(dvn: DVState)        
     {
-        forall dvn: DVState,
-               pubkey: BLSPubkey,
-               s: DVCNodeState :: 
-                    && is_honest_node(dvn, pubkey)
-                    && s == dvn.honest_nodes_states[pubkey]
-                    && !s.current_attestation_duty.isPresent()
-                    && s.latest_attestation_duty.isPresent() 
-                        ==> forall slot: Slot,
-                                   att_data: AttestationData,
-                                   bits: seq<bool>,                                   
-                                   att_shares: set<AttestationShare> ::
-                                        && slot <= s.latest_attestation_duty.safe_get().slot
-                                        && slot in s.rcvd_attestation_shares.Keys
-                                        && (att_data, bits) in s.rcvd_attestation_shares[slot].Keys
-                                        && att_data.slot == slot
-                                        && att_shares == s.rcvd_attestation_shares[slot][(att_data, bits)]
-                                        && s.construct_signed_attestation_signature(att_shares).isPresent() 
-                                        && (forall share: AttestationShare ::
-                                                share in att_shares ==> share.data == att_data )
-                                                ==> exists slashingdbAtt: SlashingDBAttestation ::
-                                                        && slashingdbAtt in s.attestation_slashing_db            
-                                                        && Some(hash_tree_root(att_data)) == slashingdbAtt.signing_root                                                                 
+        forall pubkey: BLSPubkey | is_honest_node(dvn, pubkey) ::
+            && var s := dvn.honest_nodes_states[pubkey];
+            && s.latest_attestation_duty.isPresent() 
+            && !s.current_attestation_duty.isPresent()            
+                ==> forall slot: Slot |
+                        && slot <= s.latest_attestation_duty.safe_get().slot
+                        && slot in s.rcvd_attestation_shares.Keys ::
+                                exists att_data: AttestationData,
+                                       bits: seq<bool>,                                   
+                                       att_shares: set<AttestationShare> ::                                        
+                                            && (att_data, bits) in s.rcvd_attestation_shares[slot].Keys
+                                            && att_data.slot == slot
+                                            && att_shares == s.rcvd_attestation_shares[slot][(att_data, bits)]
+                                            && s.construct_signed_attestation_signature(att_shares).isPresent() 
+                                            && (forall share: AttestationShare ::
+                                                    share in att_shares ==> share.data == att_data )
+                                                        ==> exists slashingdbAtt: SlashingDBAttestation ::
+                                                                && slashingdbAtt in s.attestation_slashing_db            
+                                                                && Some(hash_tree_root(att_data)) == slashingdbAtt.signing_root                                                                 
     }
 
-    predicate no_missing_att_in_db_cond2_in_sec_3_7<D(!new, 0)>()        
+    predicate no_missing_att_in_db_pred22_in_sec_3_7<D(!new, 0)>(dvn: DVState)        
     {
-        forall dvn: DVState,
-               pubkey: BLSPubkey,
-               s: DVCNodeState :: 
-                    && is_honest_node(dvn, pubkey)
-                    && s == dvn.honest_nodes_states[pubkey]
-                    && s.current_attestation_duty.isPresent()
-                    && s.latest_attestation_duty.isPresent() 
-                        ==> forall slot: Slot,
-                                   att_data: AttestationData,
-                                   bits: seq<bool>,                                   
-                                   att_shares: set<AttestationShare> ::
-                                        && slot < s.current_attestation_duty.safe_get().slot
-                                        && slot in s.rcvd_attestation_shares.Keys
-                                        && (att_data, bits) in s.rcvd_attestation_shares[slot].Keys
-                                        && att_data.slot == slot
-                                        && att_shares == s.rcvd_attestation_shares[slot][(att_data, bits)]
-                                        && s.construct_signed_attestation_signature(att_shares).isPresent() 
-                                        && (forall share: AttestationShare ::
-                                                share in att_shares ==> share.data == att_data )
-                                                ==> exists slashingdbAtt: SlashingDBAttestation ::
-                                                        && slashingdbAtt in s.attestation_slashing_db            
-                                                        && Some(hash_tree_root(att_data)) == slashingdbAtt.signing_root                                                                 
+        forall pubkey: BLSPubkey | is_honest_node(dvn, pubkey) ::
+            && var s := dvn.honest_nodes_states[pubkey];
+            && s.latest_attestation_duty.isPresent()                   
+                ==> forall slot: Slot |
+                        && slot <= s.latest_attestation_duty.safe_get().slot
+                        && slot in s.rcvd_attestation_shares.Keys ::
+                                exists att_data: AttestationData,
+                                       bits: seq<bool>,                                   
+                                       att_shares: set<AttestationShare> ::                                        
+                                            && (att_data, bits) in s.rcvd_attestation_shares[slot].Keys
+                                            && att_data.slot == slot
+                                            && att_shares == s.rcvd_attestation_shares[slot][(att_data, bits)]
+                                            && s.construct_signed_attestation_signature(att_shares).isPresent() 
+                                            && (forall share: AttestationShare ::
+                                                    share in att_shares ==> share.data == att_data )
+                                                        ==> exists slashingdbAtt: SlashingDBAttestation ::
+                                                                && slashingdbAtt in s.attestation_slashing_db            
+                                                                && Some(hash_tree_root(att_data)) == slashingdbAtt.signing_root                                                                 
     }
 
+/*
     predicate pred24()
     {
         forall 
@@ -381,21 +360,79 @@ module AttInvariants
                                     )
                         ) 
     }    
-
-    predicate sent_att_share_from_honest_node_in_sec_3_7<D(!new, 0)>()        
+*/
+    
+    predicate pred24(dvn: DVState)
     {
-        forall dvn: DVState, att_share: AttestationShare :: 
+        forall pubkey: BLSPubkey, att: Attestation :: 
+            && is_honest_node(dvn, pubkey)
+            && var s := dvn.honest_nodes_states[pubkey];
+            && ( exists i: nat :: 
+                    && 0 <= i 
+                    && i < |s.bn.attestations_submitted|
+                    && att == s.bn.attestations_submitted[i]
+               )
+            && ( exists att_data: AttestationData, bits: seq<bool>, k: Slot ::
+                    && k in s.rcvd_attestation_shares.Keys
+                    && (att_data, bits) in s.rcvd_attestation_shares[k].Keys
+                    && s.construct_signed_attestation_signature(
+                            s.rcvd_attestation_shares[k][(att_data, bits)]).isPresent()
+                    && att.signature == s.construct_signed_attestation_signature(
+                                            s.rcvd_attestation_shares[k][(att_data, bits)]).safe_get()
+               )
+                ==> exists pubkey1: BLSPubkey, att_data: AttestationData, bits: seq<bool>, k: Slot ::
+                        && is_honest_node(dvn, pubkey1)   
+                        && k in s.rcvd_attestation_shares.Keys
+                        && (att_data, bits) in s.rcvd_attestation_shares[k].Keys
+                        && existing_share_from_node(
+                                s.rcvd_attestation_shares[k][(att_data, bits)],
+                                att_data,
+                                s,
+                                k)           
+    } 
+
+    predicate pred25_in_sec_3_7<D(!new, 0)>(dvn: DVState)   
+    {
+        forall i: Slot, p: AttestationData -> bool | 
+            && i in dvn.consensus_on_attestation_data.Keys
+            && p in dvn.consensus_on_attestation_data[i].honest_nodes_validity_functions ::
+                forall att_data: AttestationData ::
+                    p(att_data) 
+                        ==> exists duty: AttestationDuty,    
+                                   db: set<SlashingDBAttestation>,                         
+                                   pubkey: BLSPubkey ::
+                                        && is_honest_node(dvn, pubkey)                                         
+                                        && var s := dvn.honest_nodes_states[pubkey];                                        
+                                        && duty in s.all_rcvd_duties
+                                        && consensus_is_valid_attestation_data(db, att_data, duty)
+                                        && att_data.slot == i
+                                        && db <= s.attestation_slashing_db
+                                        && forall j: Slot | 
+                                                && j <= i 
+                                                && ( exists d :: d in s.all_rcvd_duties && d.slot == j ) ::
+                                                        && dvn.consensus_on_attestation_data[j].decided_value.isPresent()
+                                                        && ( exists db_att: SlashingDBAttestation, data: AttestationData :: 
+                                                                && db_att in db
+                                                                && data.slot == j
+                                                                && db_att.signing_root == Some(hash_tree_root(data)) )
+                                                        && ( forall db_att: SlashingDBAttestation, data: AttestationData :: 
+                                                                && db_att in db
+                                                                && data.slot == j                                                                
+                                                                        ==> data == dvn.consensus_on_attestation_data[j].decided_value.safe_get() )                                                        
+    }   
+
+    
+
+    predicate sent_att_share_from_honest_node_pred26_in_sec_3_7<D(!new, 0)>(dvn: DVState)        
+    {
+        forall att_share: AttestationShare :: 
             && att_share in dvn.att_network.allMessagesSent
-            && ( exists pubkey: BLSPubkey, 
-                      s: DVCNodeState,
-                      root: Root,
-                      fork_version: Version :: 
-                            && is_honest_node(dvn, pubkey)
-                            && s == dvn.honest_nodes_states[pubkey]
-                            && fork_version == bn_get_fork_version(compute_start_slot_at_epoch(att_share.data.target.epoch))
-                            && root == compute_attestation_signing_root(att_share.data, fork_version)
-                            && att_share.signature == 
-                               rs_sign_attestation(att_share.data, 
+            && ( exists pubkey: BLSPubkey | is_honest_node(dvn, pubkey) ::
+                    && var s := dvn.honest_nodes_states[pubkey];
+                    && var epoch := compute_start_slot_at_epoch(att_share.data.target.epoch);
+                    && var fork_version := bn_get_fork_version(epoch);
+                    && var root := compute_attestation_signing_root(att_share.data, fork_version);
+                    && att_share.signature == rs_sign_attestation(att_share.data, 
                                                   fork_version, 
                                                   root, 
                                                   s.rs)
@@ -406,6 +443,29 @@ module AttInvariants
                
     }
 
+    predicate undecided_dist_consensus_instance_implies_latest_att_duty_pred27_in_sec_3_7<D(!new, 0)>(dvn: DVState)        
+    {
+        exists slot: Slot ::
+            && slot in dvn.consensus_on_attestation_data.Keys
+            && !dvn.consensus_on_attestation_data[slot].decided_value.isPresent() 
+                ==> && ( forall pubkey: BLSPubkey | is_honest_node(dvn, pubkey) ::
+                            && var s := dvn.honest_nodes_states[pubkey];
+                            && s.latest_attestation_duty.isPresent()
+                                    ==> s.latest_attestation_duty.safe_get().slot <= slot
+                       )
+    }
+
+    predicate at_most_one_undecided_dist_consensus_instance_pred28_in_sec_3_7<D(!new, 0)>(dvn: DVState)        
+    {
+        exists slot1: Slot, slot2: Slot ::
+            && slot1 in dvn.consensus_on_attestation_data.Keys
+            && slot2 in dvn.consensus_on_attestation_data.Keys
+            && !dvn.consensus_on_attestation_data[slot1].decided_value.isPresent() 
+            && !dvn.consensus_on_attestation_data[slot2].decided_value.isPresent() 
+                ==> slot1 == slot2
+    }
+
+/*
     predicate fixed_set_all_nodes_in_sec_3_7<D(!new, 0)>(
         s: DVCNodeState, 
         e: Types.Event,
@@ -414,4 +474,5 @@ module AttInvariants
     {
         s' == DVCNode_Spec.f_process_event(s, e).state ==> s.peers == s'.peers                
     }
+    */
 }
